---
title: Ch1. Logic and Proof
date: 2025-01-07 17:30:00 +/-0900
categories: [Discrete_Mathematics]
tags: [Discrete_Mathematics]     # TAG names should always be lowercase
author: Teyn
description: Learing about Logc and Proof
media_subpath: /assets/img/2025-01-07
math: true
---


# Introduction
---
Logic is the basis of all mathematical reasoning, and it has practical applications to the design of computing machines, and to other areas of computer science.
The rules of logic help in distingulishing valid from invalid mathematical arguemnts.
Proofs are essential in computer science for verifying program correctness, establishing algorithmic results, and ensuring system security.
# 1.1 Propositional Logic
---
## Proposition
---
A **Proposition** is a declarative sentence that is either true or false, but not both.
$$\begin{gathered}p : 1 + 1 = 2\\p \text{ is a proposition}\end{gathered}$$
Letters such as $p$ denote a propositional variables(or statement variables) that represent propositons
## Compound Propositions and Conditional Statements
---
**Compound Propositions** are formed from existing propositions using logical operations by combining one or more propositions.

| $p\&q$ | $p \wedge q$ | $p \vee q$  | $\neg p$ | $p \oplus q$ | $p \rightarrow q$ | $p \leftrightarrow q$ |
| :----: | :----------: | :---------: | :------: | :----------: | :---------------: | :-------------------: |
|        | Conjunction  | Disjunciton | Negation | ExclusiveOR  |    Implication    |     BiConditional     |
|  T/T   |      T       |      T      |    F     |      F       |         T         |           T           |
|  T/F   |      F       |      T      |          |      T       |         F         |           F           |
|  F/T   |      F       |      T      |    T     |      T       |         T         |           F           |
|  F/F   |      F       |      F      |          |      F       |         T         |           T           |
We will generally use parentheses to specify the order in which logical operators in a compound proposition are to be applied. The precedence of logical operators is, in order: negation($\neg$), conjunction($\wedge$) and disjunction($\vee$), implication($\rightarrow$) and biconditional($\leftrightarrow$).
Computers represent imformation using bits, and a bit is a symbol that can have two possible values representing truth values. A 1 bit represents true, and a 0 bit represents false.
# 1.2 Applicatoins of Propositional Logic
---
Statements and language in some area are imprecise or ambiguous. To make them precise, they can be translated into the language of logic.
### Example Sentence
> You can access the Internet from campus only if you are a computer science major or you are not a freshman
#### Step 1: Assign propositional variables to component propositions.
- $a$: You can access the Internet from campus
- $c$: You are a computer science major
- $f$: You are a freshman
#### Step 2: Symbolize the assertion
- $a \rightarrow (c \vee \neg f)$
System specification should be **precise, unambigiuous, and consistent.**
# 1.3 Propositional Equivalences
---
The replacement of a statement with another statement with same value is an important type of step used in a mathematical argument
Two propositions $p$ and $q$ are **logically equivalent** if $p \leftrightarrow q$ is a tautology. The notation  $p \equiv q$  denotes that $p$ and $q$ are logically equivalent.(The symbol $\Leftrightarrow$ can be used instead of $\equiv$-is not a logical connective)

|                       Equivalence                       |                                                   Equivalence                                                    | Equivalence                                             | Equivalence                                                                                                          |
| :-----------------------------------------------------: | :--------------------------------------------------------------------------------------------------------------: | :------------------------------------------------------ | -------------------------------------------------------------------------------------------------------------------- |
|     $p \wedge T \equiv p$ <br> $p \vee F \equiv p$      |                            $p\vee q \equiv q \vee p$<br> $p\wedge q\equiv q \wedge p$                            | $p \rightarrow q$<br>$\equiv \neg p \vee q$             | $(p \rightarrow q) \wedge (p \rightarrow r)$<br>$\equiv p\rightarrow (q \wedge r)$                                   |
|      $p \vee p \equiv p$ <br>$p \wedge p \equiv p$      |                           $p\vee (p \wedge q) \equiv p$<br>$p\wedge(p\vee q)\equiv p$                            | $p \rightarrow q$<br>$\equiv \neg q \rightarrow \neg p$ | $(p \rightarrow r) \wedge (q \rightarrow r)$<br>$\equiv (p \vee q)\rightarrow r$                                     |
|     $p \vee T \equiv T$ <br> $p \wedge F \equiv F$      |       $(p\vee q) \vee r \equiv p \vee (q \vee r)$ <br>$(p\wedge q) \wedge r \equiv p \wedge (q \wedge r)$        | $p \vee q$<br>$\equiv \neg p \rightarrow q$             | $p \leftrightarrow q$<br>$\equiv (p\rightarrow q) \wedge (q \rightarrow p)$                                          |
| $p \vee \neg p \equiv T$ <br>$p \wedge \neg p \equiv F$ |           $\neg(p\wedge q) \equiv \neg p \vee \neg q$ <br>$\neg(p\vee q) \equiv \neg p \wedge \neg q$            | $p \wedge q$ <br>$\equiv \neg (p \rightarrow \neg q)$   | $\neg (p \leftrightarrow q)$<br>$\equiv p \leftrightarrow \neg q$                                                    |
|                 $\neg(\neg p) \equiv p$                 | $p\vee(q\wedge r) \equiv (p \vee q)\wedge (p \vee r)$<br>$p\wedge(q\vee r) \equiv (p \wedge q)\vee (p \wedge r)$ | $\neg (p \rightarrow q)$<br>$\equiv p \wedge \neg q$    | $p \leftrightarrow q$<br>$\equiv \neg p \leftrightarrow \neg q$<br>$\equiv (p \wedge q) \vee (\neg p \wedge \neg q)$ |


A compound proposition is **satisfiable** if there is an assignement of truth values to its variables that makes it true. When no such assignments exists, the compound proposition is **unsatisfiable**.
# 1.4 Predicates and Quantifiers
---
Since propositional logic cannot adequately translate all natural language into mathematical form, predicate logic is used.
## Predicates
---
A predicate is a logical expression that includes one or more variables, and when specific values are assigned to these variables, it generates a proposition that is either true or false.
$$\begin{gathered}P(x, y): x\text{ is greater than }y\\P(3, 2)\text{ is the statement "3>2", which is true}\\P(2, 3)\text{ is the statement "2>3", which is false}\end{gathered}$$

## Quantifiers
---
When all the variables in a propositional function are assigned values, the resulting statement becomes a proposition with a certain truth value.
There are two types of quantification
$$\begin{align}\text{1. }& \text{Universal quantification($\forall$):  A predicate is true for every element under consideration}\\\text{2. }&\text{Existential quantification($\exists$): There is one or more element under consideration for }\\&\,\,\,\,\,\,\,\,\,\,\,\,\,\,\,\,\,\,\,\,\,\,\,\,\,\,\,\,\,\,\,\,\,\,\,\,\,\,\,\,\,\,\,\,\,\,\,\,\,\,\,\,\,\,\,\,\,\,\,\,\,\,\,\,\,\,\,\,\,\,\,\,\,\,\,\,\,\,\text{which the predicate is true.}\\\text{3. }& \text{Uniqueness quantification($\exists!$): There is exactly one element under consideration.}\end{align}$$
The quantifiers have higher precedence than all logical operators from propositional calculus.
All variables in a propositional function **must be bound or set equal to a particular value**. This can be done by a combination of quantifiers and value assignment.
**A statement with free variable is not a proposition.**
## Logically Equivalent
---
Statements involving predicates and quantifiers are **logically equivalent** if and only if they have the same truth value no matter which predicates are substituted into these statements and which domain of discourse is used for the variables in these propositional functions.
We use the notation $S \equiv T$ to indicate that two statements $S$ and $T$ involving predicates and quantifiers are logically equivalent.
## Negating Quantified Expressions
---

| Negation             | Equivalent statement  | When Negation True?                        | When False?                              |
| :------------------- | :-------------------- | :----------------------------------------- | :--------------------------------------- |
| $\neg \exists xP(x)$ | $\forall x \neg P(x)$ | For every $x$, $P(x)$ is false.            | There is an $x$ for which $P(x)$ is true |
| $\neg \forall xP(x)$ | $\exists x \neg P(x)$ | There is an $x$ for which $P(x)$ is false. | $P(x)$ is true for every $x$             |
# 1.5 Nested Quantifiers
---
**Nested Quantifiers** refer to situations in logic where one quantifier occurs within the scope of another quantifier. This allows for more complex logical expressions by spcifying how multiple variables are related through different quantifers. Nested quantifiers are used to express statements involving multiple vairables, Where the scope of one quantifier directly affects the other.

| Statement                   | When True?                                                | When False?                                               |
| :-------------------------- | :-------------------------------------------------------- | :-------------------------------------------------------- |
| $\forall x \forall yP(x,y)$ | $P(x,y)$ is true for every pair $x, y$.                   | There is a pair $x,y$ for which $P(x,y)$ is false.        |
| $\forall x \exists yP(x,y)$ | For every $x$ there is a $y$ for which $P(x,y)$ is true.  | There is an $x$ such that $P(x,y)$ is false for every $y$ |
| $\exists x \forall yP(x,y)$ | There is an $x$ for which $P(x,y)$ is true for every $y$. | For every $x$ there is a $y$ for which $P(x,y)$ is false  |
| $\exists x \exists yP(x,y)$ | There is a pair $x,y$ for which $P(x,y)$ is ture.         | $P(x,y)$ is false for every pair $x, y$.                  |
# 1.6 Rules of Inference
---
## Validity
---
The validity of an arguments holds when the conclusion is true of all variables that make the premises true.
$$\begin{align}\text{Note> }&\text{An argument is expressed as an implication. For the implication to be true,}\\&\text{either the premises and conclusion must be true. or the premises must be false.}\\&\text{$\therefore$ if an argument is valid, the proposition is a tautology.}\end{align}$$
## Rules of Inference
---
To show validity of an argument from the perspective of propositional logic, show that arguement form is valid. To demonstrate the validity of an argument with multiple overlapping propositions, using a truth table involves too many cases, so 
simple argument forms, called rules of inference are used.

| Name                  | Tautology                                                               | Rule of Inference                                                                       | Name                   | Tautology                                                                                               | Rule of Inference                                                                                     |
| --------------------- | ----------------------------------------------------------------------- | --------------------------------------------------------------------------------------- | ---------------------- | ------------------------------------------------------------------------------------------------------- | ----------------------------------------------------------------------------------------------------- |
| Modus ponens          | $\begin{align}&(p\wedge (p \rightarrow q)) \\&\rightarrow q\end{align}$ | $\begin{align}&p\\&\underline{p\rightarrow q}\\\therefore &\,q\end{align}$              | Modus tollens          | $\begin{align}&(\neg q \wedge(p \rightarrow q)) \\&\rightarrow \neg p\end{align}$                       | $\begin{align}&\neg q\\&\underline{p\rightarrow q}\\\therefore &\,\neg p\end{align}$                  |
| Disjunctive syllogism | $\begin{align}&((p\vee q) \wedge \neg p) \\&\rightarrow q\end{align}$   | $\begin{align}&p \vee q\\&\underline{\neg p\,\,\,\,\,\,\,}\\\therefore &\,q\end{align}$ | Hypothetical syllogism | $\begin{align}&((p\rightarrow q) \wedge (q \rightarrow r)) \\&\rightarrow (p \rightarrow r)\end{align}$ | $\begin{align}&p\rightarrow q\\&\underline{q\rightarrow r}\\\therefore &\,p \rightarrow r\end{align}$ |
| Addition              | $p \rightarrow (p \vee q)$                                              | $\begin{align}&\underline{p\,\,\,\,\,\,\,\,\,\,}\\\therefore & \,p\vee q\end{align}$    | Simplification         | $(p \wedge q) \rightarrow p$                                                                            | $\begin{align}&\underline{p \wedge q}\\\therefore & \,p\end{align}$                                   |
| Conjuction            | $\begin{align}&((p) \wedge (q)) \\&\rightarrow (p \wedge q)\end{align}$ | $\begin{align}&p\\&\underline{q\,\,\,\,\,\,\,\,}\\\therefore &\,p \wedge q\end{align}$  | Resolution             | $\begin{align}&((p \vee q) \wedge (\neg p \vee r))\\&\rightarrow (q \vee r)\end{align}$                 | $\begin{align}&p \vee q\\&\underline{\neg p \vee r}\\\therefore &\,q \vee r\end{align}$               |
### Resolution Example
$$\begin{align}&[(p \wedge q) \vee r ] \wedge [r \rightarrow s]
\\&\equiv (p \vee r) \wedge [(q \vee r) \wedge (\neg r \vee s)]
\\&\equiv p \vee s\end{align}$$
### Rules for Inference for Quantified Statements
| Name                      | Rule of Inference                                                                                                                                                              | Name                       | Rule of Inference                                                                                   |
| ------------------------- | ------------------------------------------------------------------------------------------------------------------------------------------------------------------------------ | -------------------------- | --------------------------------------------------------------------------------------------------- |
| Universal instantiation   | $\begin{align}&\underline{\forall x P(x)}\\\therefore &\,P(c)\end{align}$                                                                                                      | Universal generalization   | $\begin{align}&\underline{P(c) \text{ for an arbitrary } c}\\\therefore &\,\forall P(x)\end{align}$ |
| Existential instantiation | $\begin{align}&\underline{\exists x P(x)\,\,\,\,\,\,\,\,\,\,\,\,\,\,\,\,\,\,\,\,\,\,\,\,\,\,\,\,\,\,\,\,\,\,\,\,\,}\\\therefore &\,P(c) \text{ for some element }c\end{align}$ | Existential generalization | $\begin{align}&\underline{P(c) \text{ for some element } c}\\\therefore &\,\exists P(x)\end{align}$ |
## Fallacies
---
### The fallacy of affirming the conclusion
- Form: $[(p \rightarrow q) \wedge q] \rightarrow p$
- This argument is not a tautology and therefore not a rule of inference.
### The fallacy of denying the hypothesis
- Form: $[(p \rightarrow q) \wedge \neg p] \rightarrow \neg q$
- This argument is also not a tautology and hence not a rule of inference.
# 1.8 Introduction to Proofs
---
## Necessity and Terms
___
A proof is a valid argument that establishes the truth of a mathematical statement. A proof can use the hypotheses of the theorem, axioms assumed to be true, previously proven theorems.
- A **Theorem** is a statement that can be shown to be true
	- Axioms(or postulates): Statements we assume to be true
	- The 
## Methods of Proving Theorems
---
### Direct Proofs
---
1. Assume that $p$ is true.
2. Show that $q$ must also be true by using axioms, definitions, previously proven theorems, together with rules of inference.
### Indirect Proofs
---
#### Proof by contraposition
---
1. Take $\neg q$ as a hypothesis.
2. Use axioms, definitions, previously proven theorems, together with rules of inference.
3. Establish the premise the premise $p$ is false(=$\neg p$ is true)
#### Proof by Contradiction
---
1. Assume that $q$ is false, and $p \rightarrow \neg q$ is true.
2. Derive a contradiction, usually of the form $r\wedge \neg r$, which establishes $(p \rightarrow \neg q) \rightarrow (r \wedge \neg r)$
3. Then the proposition $(p \rightarrow \neg q)$ is must be false. 
4. Consequently, $(p \rightarrow q)$ must be true.
### Vacuous & Trivial Proof
---
Vacuous: The conditional statement $p \rightarrow q$ can be proved by showing that $p$ is false.
Trivial : The conditional statement $p \rightarrow q$ can be proved by showing that its $q$ is true.

